major update
1. Change char type from `T` to `T -> Prop` with respect to relational style.
   Make Record arguments explicit.

2. Refactor PreGraph operations into Record.
   Fix `char_step` definitions.
   Remove multiple unused definitions.

3. Refactor PreGraph concatenative relations into Record (as product type).

4. Add Notation, Local Scope for Record definitions.

5. Remove CertiGraph dependency.

6. Update monadlib dependency to fix rule pattern.

lib/PreGraph.v
@@ -1,4 +1,3 @@
-Require Import CertiGraph.lib.Ensembles_ext.
 Require Import Coq.ZArith.ZArith.
 Require Import Coq.Classes.RelationClasses.
 From SetsClass Require Import SetsClass.
@@ -10,23 +9,185 @@ Import SetsNotation.
 Local Open Scope Z_scope.
 Local Open Scope sets_scope.
 
-Definition epsilon {T: Type} : option T := None.
+(** Set relations *)
 
-Section GRAPH_DEF.
+Definition Sets_disjoint_union {X: Type} (A B C: X -> Prop): Prop :=
+  A ∩ B == ∅ /\
+  A ∪ B == C.
 
-Record PreGraph {Vertex Edge: Type} := {
-  vvalid : Ensemble Vertex;
-  evalid : Ensemble Edge;
+Definition Sets_overlap {X: Type} (A B: X -> Prop): Prop :=
+  exists x, x ∈ A /\ x ∈ B.
+
+Module Graph.
+
+Record PreGraph (Vertex Edge: Type) := {
+  vvalid : Vertex -> Prop;
+  evalid : Edge -> Prop;
   src : Edge -> Vertex;
   dst : Edge -> Vertex
 }.
 
+Notation "pg '.(vvalid)'" := (vvalid _ _ pg) (at level 1).
+Notation "pg '.(evalid)'" := (evalid _ _ pg) (at level 1).
+Notation "pg '.(src)'" := (src _ _ pg) (at level 1).
+Notation "pg '.(dst)'" := (dst _ _ pg) (at level 1).
+
+Record step_aux {V E: Type} (pg: PreGraph V E) (e: E) (x y: V): Prop :=
+{
+  step_evalid: pg.(evalid) e;
+  step_src_valid: pg.(vvalid) x;
+  step_dst_valid: pg.(vvalid) y;
+  step_src: pg.(src) e = x;
+  step_dst: pg.(dst) e = y;
+}.
+
+Definition step {V E: Type} (pg: PreGraph V E) (x y: V): Prop :=
+  exists e, step_aux pg e x y.
+
+Record add_vertex {V E} (g1: PreGraph V E) (v: V) (g2: PreGraph V E): Prop :=
+{
+  add_vertex_vertex:
+    Sets_disjoint_union g1.(vvalid) (Sets.singleton v) g2.(vvalid);
+  add_vertex_edge:
+    g1.(evalid) == g2.(evalid);
+  add_vertex_src:
+    forall e, e ∈ g1.(evalid) -> g2.(src) e = g1.(src) e;
+  add_vertex_dst:
+    forall e, e ∈ g1.(evalid) -> g2.(dst) e = g1.(dst) e;
+}.
+
+Record add_edge {V E} (g1: PreGraph V E) (e0: E) (x y: V) (g2: PreGraph V E): Prop :=
+{
+  add_edge_vertex:
+    g1.(vvalid) == g2.(vvalid);
+  add_edge_edge:
+    Sets_disjoint_union g1.(evalid) (Sets.singleton e0) g2.(evalid);
+  add_edge_src_old:
+    forall e, e ∈ g1.(evalid) -> g2.(src) e = g1.(src) e;
+  add_edge_dst_old:
+    forall e, e ∈ g1.(evalid) -> g2.(dst) e = g1.(dst) e;
+  add_edge_src_new: g2.(src) e0 = x;
+  add_edge_dst_new: g2.(dst) e0 = y;
+}.
+
+(* disjoint union *)
+Record union_rel {V E} (g1 g2 g: PreGraph V E): Prop :=
+{
+  union_vertex: Sets_disjoint_union g1.(vvalid) g2.(vvalid) g.(vvalid);
+  union_edge: Sets_disjoint_union g1.(evalid) g2.(evalid) g.(evalid);
+  union_src1: forall e, e ∈ g1.(evalid) -> g.(src) e = g1.(src) e;
+  union_src2: forall e, e ∈ g2.(evalid) -> g.(src) e = g2.(src) e;
+  union_dst1: forall e, e ∈ g1.(evalid) -> g.(dst) e = g1.(dst) e;
+  union_dst2: forall e, e ∈ g2.(evalid) -> g.(dst) e = g2.(dst) e;
+}.
+
+End Graph.
+
+Notation "'PreGraph'" := (Graph.PreGraph) (at level 0).
+Notation "pg '.(vvalid)'" := (Graph.vvalid _ _ pg) (at level 1).
+Notation "pg '.(evalid)'" := (Graph.evalid _ _ pg) (at level 1).
+Notation "pg '.(src)'" := (Graph.src _ _ pg) (at level 1).
+Notation "pg '.(dst)'" := (Graph.dst _ _ pg) (at level 1).
+
+
+(** NFA definition *)
+
+Section PG_NFA.
+
+Definition epsilon {T: Type} : option T := None.
+
 (* We use Z as unique label for each vertex and edge. *)
 (* And use `symbol` to record character on each edge based on label. *)
-Record pg_nfa {T: Type} := {
-  pg : @PreGraph Z Z;
-  symbol : Z -> option T
+(** represent multi-edge symbol(s) as symbol set *)
+Record pg_nfa (T: Type) := {
+  pg : PreGraph Z Z;
+  symbol : Z -> option (T -> Prop)
 }.
+
+Notation "g '.(pg)'" := (pg _ g) (at level 1).
+Notation "g '.(symbol)'" := (symbol _ g) (at level 1).
+
+Record add_vertex {T} (g1: pg_nfa T) (v: Z) (g2: pg_nfa T): Prop :=
+{
+  add_vertex_pg:
+    Graph.add_vertex g1.(pg) v g2.(pg);
+  add_vertex_symbol:
+    forall e, e ∈ g1.(pg).(evalid) -> g2.(symbol) e = g1.(symbol) e;
+}.
+
+Record add_edge {T} (g1: pg_nfa T) (e0 x y: Z) t (g2: pg_nfa T): Prop :=
+{
+  add_edge_pg:
+    Graph.add_edge g1.(pg) e0 x y g2.(pg);
+  add_edge_symbol_old:
+    forall e, e ∈ g1.(pg).(evalid) -> g2.(symbol) e = g1.(symbol) e;
+  add_edge_symbol_new:
+    g2.(symbol) e0 = t;
+}.
+
+Record union_rel {T} (g1 g2 g: pg_nfa T): Prop :=
+{
+  union_pg: Graph.union_rel g1.(pg) g2.(pg) g.(pg);
+  union_symbol1: forall e, e ∈ g1.(pg).(evalid) -> g.(symbol) e = g1.(symbol) e;
+  union_symbol2: forall e, e ∈ g2.(pg).(evalid) -> g.(symbol) e = g2.(symbol) e;
+}.
+
+Definition empty_nfa {T: Type} : pg_nfa T := {|
+  (* ? Pose src/dst as `fun n => -1` to indicate emptyness *)
+  pg := @Graph.Build_PreGraph Z Z (fun v => False) (fun e => False) (fun n => (-1)%Z) (fun n => (-1)%Z);
+  symbol := fun _ => None
+|}.
+
+Definition emptyset_nfa {T: Type} (v1 v2 : Z) : pg_nfa T := {|
+  (* ? Pose src/dst as `fun n => -1` to indicate emptyness *)
+  pg := @Graph.Build_PreGraph Z Z (fun v => v = v1 \/ v = v2) (fun e => False) (fun n => (-1)%Z) (fun n => (-1)%Z);
+  symbol := fun _ => None
+|}.
+
+Definition e_step {T} (G: pg_nfa T) : Z -> Z -> Prop :=
+  fun x y => exists e, Graph.step_aux G.(pg) e x y /\ G.(symbol) e = None.
+
+Definition e_steps {T} (G: pg_nfa T) : Z -> Z -> Prop :=
+  clos_refl_trans (e_step G).
+
+Definition c_step {T} (G: pg_nfa T) (c: T) : Z -> Z -> Prop :=
+  fun x y =>
+    (* t: T -> Prop *)
+    exists e t, Graph.step_aux G.(pg) e x y /\ G.(symbol) e = Some t /\ c ∈ t.
+
+(** FIX *)
+Definition char_step {T} (G: pg_nfa T) (c: T) : Z -> Z -> Prop :=
+  (c_step G c) ∘ (e_steps G).
+
+(** FIX *)
+Fixpoint string_step {T} (G: pg_nfa T) (l: list T) : Z -> Z -> Prop :=
+  match l with
+  | nil => e_steps G
+  | cons s l' => (string_step G l') ∘ (char_step G s)
+  end.
+
+Definition G_match_str {T} (G: pg_nfa T) (sv ev: Z) (l: list T)
+  : Prop := string_step G l sv ev.
+
+End PG_NFA.
+
+(** Reserved relations for DFA representation *)
+
+(* Calculate the new e_closure when consuming a char *)
+Definition closure_step {T} (G: pg_nfa T) (ec: Z -> Prop) (c: T) : Z -> Prop :=
+  fun y => exists x, ec x /\ c_step G c x y.
+
+Fixpoint nfa_closure {T} (G: pg_nfa T) (ec: Z -> Prop) (l: list T) : Z -> Prop :=
+  match l with
+  | nil => ec
+  | cons s l' => nfa_closure G (closure_step G ec s) l'
+  end.
+
+Definition G_match_string {T} (G: pg_nfa T) (sv ev: Z) (l: list T) : Prop :=
+  (nfa_closure G (e_steps G sv) l) ev.
+
+
+Section NFA_REL.
 
 (* state without graph *)
 Record state := {
@@ -34,162 +195,46 @@ Record state := {
   max_e : Z
 }.
 
-Record elem {T: Type} := {
+Record elem (T: Type) := {
   startVertex : Z;
   endVertex : Z;
-  graph : @pg_nfa T;
+  graph : pg_nfa T;
 }.
 
 (* state with graph *)
-Record state' {T} := {
+Record state' (T: Type) := {
   max_v' : Z;
   max_e' : Z;
-  st_graph : @pg_nfa T
+  st_graph : pg_nfa T
 }.
-
-(* Record elem' := {
-  startVertex' : Z;
-  endVertex' : Z
-}. *)
 
 Definition elem' : Type := (Z * Z)%type.
 
-Definition addValidFunc {T: Type} (v: T) (validFunc: Ensemble T) : Ensemble T :=
-  fun n => validFunc n \/ n = v.
-
-Definition updateEdgeFunc (edgeFunc: Z -> Z) (e: Z) (v: Z) :
-  Z -> Z := fun n => if Z.eqb e n then v else edgeFunc n.
-
-Definition removeValidFunc {T: Type} (v: T) (validFunc: Ensemble T) : Ensemble T :=
-  fun n => validFunc n /\ n <> v.
-
-Inductive step (pg: @PreGraph Z Z): Z -> Z -> Prop :=
-  | step_intro: forall e x y, evalid pg e -> src pg e = x -> dst pg e = y -> step pg x y.
-
-Definition edge (pg : @PreGraph Z Z) (n n' : Z) : Prop :=
-  vvalid pg n /\ vvalid pg n' /\ step pg n n'.
-
-Definition vertex_overlap {T: Type} : @pg_nfa T -> @pg_nfa T -> Prop :=
-  fun g1 g2 =>
-    exists v, vvalid g1.(pg) v /\ vvalid g2.(pg) v.
-
-Definition edge_overlap {T} : @pg_nfa T -> @pg_nfa T -> Prop :=
-  fun g1 g2 => exists v v', edge g1.(pg) v v' /\ edge g2.(pg) v v'.
-
-Definition symbol_overlap {T} : @pg_nfa T -> @pg_nfa T -> Prop :=
-  fun g1 g2 => exists e c1 c2, g1.(symbol) e = Some c1 /\ g2.(symbol) e = Some c2.
-
-Definition G_add_vertex {T} : @pg_nfa T -> Z -> @pg_nfa T -> Prop :=
-  fun G1 n G2 =>
-    let g1 := G1.(pg) in
-    let g2 := G2.(pg) in
-    (~ vvalid g1 n) /\
-    (forall v, g2.(vvalid) v <-> g1.(vvalid) v \/ v = n) /\
-    (forall e, evalid g2 e <-> evalid g1 e) /\
-    (forall e, g2.(src) e = g1.(src) e) /\
-    (forall e, g2.(dst) e = g1.(dst) e) /\
-    (forall e, G2.(symbol) e = G1.(symbol) e).
-
-Definition G_add_edge {T} : pg_nfa -> Z -> Z -> Z -> option T -> pg_nfa -> Prop :=
-  fun G1 n s t c G2 =>
-    let g1 := G1.(pg) in
-    let g2 := G2.(pg) in
-    (g1.(vvalid) s /\ g1.(vvalid) t) /\
-    (forall v, g2.(vvalid) v <-> g1.(vvalid) v) /\
-    (~ g1.(evalid) n) /\
-    (forall e, g2.(evalid) e <-> g1.(evalid) e \/ e = n) /\
-    (forall e, g2.(src) e = g1.(src) e) /\
-    (forall e, g2.(dst) e = g1.(dst) e) /\
-    (forall e, G2.(symbol) e = if Z.eqb e n then c else G1.(symbol) e).
-
-(* disjoint *)
-Definition G_union_rel {T} : @pg_nfa T -> @pg_nfa T -> @pg_nfa T -> Prop :=
-  fun g1 g2 g =>
-    (forall v, vvalid g1.(pg) v \/ vvalid g2.(pg) v <-> vvalid g.(pg) v) /\
-    (forall e, evalid g1.(pg) e \/ evalid g2.(pg) e <-> evalid g.(pg) e) /\
-    (forall e, src g.(pg) e = if src g1.(pg) e >? 0
-                              then src g1.(pg) e
-                              else src g2.(pg) e) /\
-    (forall e, dst g.(pg) e = if dst g1.(pg) e >? 0
-                              then dst g1.(pg) e
-                              else dst g2.(pg) e) /\
-    (forall e, symbol g e = match symbol g1 e with
-                            | Some c1 => Some c1
-                            | None => symbol g2 e
-                            end).
-
-Definition G_disjoint {T} : @pg_nfa T -> @pg_nfa T -> Prop :=
-  fun G1 G2 =>
-    let g1 := G1.(pg) in
-    let g2 := G2.(pg) in
-    (forall v, g1.(vvalid) v /\ g2.(vvalid) v -> False) /\
-    (forall e, g1.(evalid) e /\ g2.(evalid) e -> False).
-
-End GRAPH_DEF.
-
-Section GRAPH_EXAMPLE.
-
-Definition empty_nfa {T: Type} : @pg_nfa T := {|
-  (* ? Pose src/dst as `fun n => -1` to indicate emptyness *)
-  pg := @Build_PreGraph Z Z (fun v => False) (fun e => False) (fun n => (-1)%Z) (fun n => (-1)%Z);
-  symbol := fun _ => None
-|}.
-
-Definition emptyset_nfa {T: Type} (v1 v2 : Z) : @pg_nfa T := {|
-  (* ? Pose src/dst as `fun n => -1` to indicate emptyness *)
-  pg := @Build_PreGraph Z Z (fun v => v = v1 \/ v = v2) (fun e => False) (fun n => (-1)%Z) (fun n => (-1)%Z);
-  symbol := fun _ => None
-|}.
-
-End GRAPH_EXAMPLE.
-
-Section NFA_REL.
-
-Definition e_step {T} (G: @pg_nfa T) : Z -> Z -> Prop :=
-  fun x y => exists e, step G.(pg) x y /\ G.(symbol) e = None.
-
-Definition e_steps {T} (G: @pg_nfa T) : Z -> Z -> Prop :=
-  (** See SetsClass *)
-  clos_refl_trans (e_step G).
-(** TODO: SetsClass induction_1n transitivity_1n one_step vs n_step *)
-(** rel *)
-
-(** T -> rel *)
-(** string_step : rel concat  *)
-(** G_match_str := string_step + e_closure *)
-
-(* ? *)
-Definition c_step {T} (G: @pg_nfa T) (c: T) : Z -> Z -> Prop :=
-  fun x y => exists e, step G.(pg) x y /\ G.(symbol) e = Some c.
-
-Definition char_step {T} (G: @pg_nfa T) (c: T) : Z -> Z -> Prop :=
-  (e_steps G) ∘ (c_step G c) ∘ (e_steps G).
-
-Fixpoint string_step {T} (G: @pg_nfa T) (l: list T) : Z -> Z -> Prop :=
-  match l with
-  | nil => Rels.id
-  | cons s l' => (char_step G s) ∘ (string_step G l')
-  end.
-
-Definition G_match_str {T} (G: @pg_nfa T) (sv ev: Z) (l: list T)
-  : Prop := string_step G l sv ev.
-
-
-
-(** Calculate the new e_closure when consuming a char *)
-Definition closure_step {T} (G: @pg_nfa T) (ec: Z -> Prop) (c: T) : Z -> Prop :=
-  fun y => exists x, ec x /\ c_step G c x y.
-
-Fixpoint nfa_closure {T} (G: @pg_nfa T) (ec: Z -> Prop) (l: list T) : Z -> Prop :=
-  match l with
-  | nil => ec
-  | cons s l' => nfa_closure G (closure_step G ec s) l'
-  end.
-
-Definition G_match_string {T} (G: @pg_nfa T) (sv ev: Z) (l: list T) : Prop :=
-  (nfa_closure G (e_steps G sv) l) ev.
-
 End NFA_REL.
 
-(* step (epsilon / char) ; reflexive transitive closure *)
-(* monad repeatBreak whileBreak *)
+Module PreGraphNotations.
+
+Declare Scope pg_scope.
+Delimit Scope pg_scope with pg.
+
+Notation "'PreGraph'" := (Graph.PreGraph) (at level 0).
+Notation "pg '.(vvalid)'" := (Graph.vvalid _ _ pg) (at level 1).
+Notation "pg '.(evalid)'" := (Graph.evalid _ _ pg) (at level 1).
+Notation "pg '.(src)'" := (Graph.src _ _ pg) (at level 1).
+Notation "pg '.(dst)'" := (Graph.dst _ _ pg) (at level 1).
+
+Notation "g '.(pg)'" := (pg _ g) (at level 1).
+Notation "g '.(symbol)'" := (symbol _ g) (at level 1).
+
+Notation "s '.(max_v)'" := (max_v s) (at level 1).
+Notation "s '.(max_e)'" := (max_e s) (at level 1).
+
+Notation "el '.(startVertex)'" := (startVertex _ el) (at level 1).
+Notation "el '.(endVertex)'" := (endVertex _ el) (at level 1).
+Notation "el '.(graph)'" := (graph _ el) (at level 1).
+
+Notation "s '.(max_v')'" := (max_v' _ s) (at level 1).
+Notation "s '.(max_e')'" := (max_e' _ s) (at level 1).
+Notation "s '.(st_graph)'" := (st_graph _ s) (at level 1).
+
+End PreGraphNotations.
