theories/st_graph_nfa.v
@@ -2,20 +2,20 @@ Require Import Regex2NFA.lib.PreGraph.
 Require Import Regex2NFA.theories.regex.
 Require Import Coq.Init.Datatypes.
 Require Import Coq.ZArith.ZArith.
+From SetsClass Require Import SetsClass.
 From StateMonad.monaderror Require Import monadEbasic.
 
 Import MonadwitherrDeno.
 Import MonadNotation.
+Import PreGraphNotations.
 Local Open Scope Z_scope.
 Local Open Scope stmonad_scope.
-
-Section Graph_NFA_DEF.
+Local Open Scope pg_scope.
 
 (** program state' (sv, ev) *)
 
-Definition get_new_vertex' {T} : program (@state' T) Z := {|
-  nrm :=
-    fun s1 n s2 =>
+Definition get_new_vertex' {T} : program (state' T) Z := {|
+  nrm := fun s1 n s2 =>
     s2.(max_v') = s1.(max_v') + 1 /\
     s2.(max_e') = s1.(max_e') /\
     n = s2.(max_v') /\
@@ -23,131 +23,84 @@ Definition get_new_vertex' {T} : program (@state' T) Z := {|
   err := fun s1 => False (* no error case *)
 |}.
 
-Definition get_new_edge' {T} : program (@state' T) Z := {|
+Definition get_new_edge' {T} : program (state' T) Z := {|
   nrm :=
     fun s1 n s2 =>
     s2.(max_v') = s1.(max_v') /\
     s2.(max_e') = s1.(max_e') + 1 /\
-    n = s2.(max_v') /\
+    n = s2.(max_e') /\
     s2.(st_graph) = s1.(st_graph);
   err := fun s1 => False (* no error case *)
 |}.
 
-Definition pregraph_add_vertex' {T} (v: Z) : program (@state' T) pg_nfa := {|
-  nrm :=
-    fun s1 G s2 =>
+Definition G_add_vertex' {T} : program (state' T) Z := {|
+  nrm := fun s1 n s2 =>
+    let G1 := s1.(st_graph) in
+    let G2 := s2.(st_graph) in
+    s2.(max_v') = s1.(max_v') + 1 /\
+    s2.(max_e') = s1.(max_e') /\
+    add_vertex G1 s2.(max_v') G2 /\
+    n = s2.(max_v');
+  err := fun s1 => False (* no error case *)
+|}.
+
+Definition G_add_edge' {T} (x y: Z) t : program (state' T) Z := {|
+  nrm := fun s1 n s2 =>
     let G1 := s1.(st_graph) in
     let G2 := s2.(st_graph) in
     s2.(max_v') = s1.(max_v') /\
-    s2.(max_e') = s1.(max_e') /\
-    G_add_vertex G1 v G2 /\
-    G = G2;
-  err := fun s1 => v <> s1.(max_v')
-  (* error if new vertex label mismatches current state *)
+    s2.(max_e') = s1.(max_e') + 1 /\
+    add_edge G1 s2.(max_e') x y t G2 /\
+    n = s2.(max_e');
+  err := fun s1 => False (* error if edge exists *)
+  (*? or  *)
 |}.
-
-Definition pregraph_add_edge' {T} (e: Z) (s t: Z) (c : option T)
-: program (@state' T) pg_nfa := {|
-  nrm :=
-    fun s1 G s2 =>
-    let G1 := s1.(st_graph) in
-    let G2 := s2.(st_graph) in
-    s2.(max_v') = s1.(max_v') /\
-    s2.(max_e') = s1.(max_e') /\
-    G_add_edge G1 e s t c G2 /\
-    G = G2;
-  err :=
-    fun s1 =>
-    let g1 := s1.(st_graph).(pg) in
-    exists e',
-    g1.(vvalid) s /\ g1.(vvalid) t /\
-    g1.(evalid) e' /\
-    g1.(src) e' = s /\
-    g1.(dst) e' = t
-  (* error if edge exists *)
-|}.
-
-(* Definition pregraph_add_whole_vertex' {T}
-: program (@state' T) pg_nfa :=
-  v <- get_new_vertex' ;;
-  pregraph_add_vertex' v. *)
-
-Definition pregraph_add_whole_edge' {T} (s t: Z) (c: option T)
-: program state' pg_nfa :=
-  e <- get_new_edge' ;;
-  pregraph_add_edge' e s t c.
-
-(* Definition nfa_to_elem' {T} (sv ev: Z) : program (@state' T) elem' := {|
-  nrm :=
-    fun s1 E s2 =>
-    s1 = s2 /\
-    E = {|
-      startVertex' := sv;
-      endVertex' := ev;
-    |};
-  err :=
-    fun s1 =>
-    let g := s1.(st_graph) in
-    ~ vvalid g.(pg) sv \/ ~ vvalid g.(pg) ev
-|}. *)
 
 Fixpoint regexToNFA' {T} (r : reg_exp T)
-: program state' elem' :=
+: program (state' T) elem' :=
   match r with
   | EmptySet_r =>
-    v1 <- get_new_vertex' ;;
-    pregraph_add_vertex' v1 ;;
-    v2 <- get_new_vertex' ;;
-    pregraph_add_vertex' v2 ;;
+    v1 <- G_add_vertex' ;;
+    v2 <- G_add_vertex' ;;
     return (v1, v2)
 
   | EmptyStr_r =>
-    v1 <- get_new_vertex' ;;
-    pregraph_add_vertex' v1 ;;
-    v2 <- get_new_vertex' ;;
-    pregraph_add_vertex' v2 ;;
-    pregraph_add_whole_edge' v1 v2 None ;;
+    v1 <- G_add_vertex' ;;
+    v2 <- G_add_vertex' ;;
+    G_add_edge' v1 v2 epsilon ;;
     return (v1, v2)
 
   | Char_r t =>
-    v1 <- get_new_vertex' ;;
-    pregraph_add_vertex' v1 ;;
-    v2 <- get_new_vertex' ;;
-    pregraph_add_vertex' v2 ;;
-    pregraph_add_whole_edge' v1 v2 (Some t) ;;
+    v1 <- G_add_vertex' ;;
+    v2 <- G_add_vertex' ;;
+    G_add_edge' v1 v2 (Some t) ;;
     return (v1, v2)
 
   | Concat_r r1 r2 =>
     '(sv1, ev1) <- regexToNFA' r1 ;;
     '(sv2, ev2) <- regexToNFA' r2 ;;
-    pregraph_add_whole_edge' ev1 ev2 epsilon ;;
+    G_add_edge' ev1 ev2 epsilon ;;
     return (sv1, ev2)
 
   | Union_r r1 r2 =>
     '(sv1, ev1) <- regexToNFA' r1 ;;
     '(sv2, ev2) <- regexToNFA' r2 ;;
-    v1 <- get_new_vertex' ;;
-    pregraph_add_vertex' v1 ;;
-    v2 <- get_new_vertex' ;;
-    pregraph_add_vertex' v2 ;;
-    pregraph_add_whole_edge' v1 sv1 epsilon ;;
-    pregraph_add_whole_edge' v1 sv2 epsilon ;;
-    pregraph_add_whole_edge' ev1 v2 epsilon ;;
-    pregraph_add_whole_edge' ev2 v2 epsilon ;;
+    v1 <- G_add_vertex' ;;
+    v2 <- G_add_vertex' ;;
+    G_add_edge' ev1 ev2 epsilon ;;
+    G_add_edge' v1 sv2 epsilon ;;
+    G_add_edge' ev1 v2 epsilon ;;
+    G_add_edge' ev2 v2 epsilon ;;
     return (v1, v2)
 
   | Star_r r =>
     '(sv, ev) <- regexToNFA' r ;;
-    v1 <- get_new_vertex' ;;
-    pregraph_add_vertex' v1 ;;
-    v2 <- get_new_vertex' ;;
-    pregraph_add_vertex' v2 ;;
-    pregraph_add_whole_edge' v1 ev epsilon ;;
-    pregraph_add_whole_edge' ev v2 epsilon ;;
-    pregraph_add_whole_edge' ev sv epsilon ;;
+    v1 <- G_add_vertex' ;;
+    v2 <- G_add_vertex' ;;
+    G_add_edge' v1 ev epsilon ;;
+    G_add_edge' ev v2 epsilon ;;
+    G_add_edge' ev sv epsilon ;;
     return (v1, v2)
   end.
 
 (** recursion *)
-
-End Graph_NFA_DEF.
