theories/st_nograph_nfa.v
@@ -4,41 +4,33 @@ Require Import Coq.Init.Datatypes.
 Require Import Coq.ZArith.ZArith.
 Require Import Coq.Strings.Ascii.
 Require Import List.
+From SetsClass Require Import SetsClass.
 From StateMonad.monaderror Require Import monadEbasic.
 
 Import MonadwitherrDeno.
 Import MonadNotation.
 Import ListNotations.
+Import SetsNotation.
+Import PreGraphNotations.
 Local Open Scope Z_scope.
 Local Open Scope stmonad_scope.
-
-Section NoGraph_NFA_DEF.
+Local Open Scope sets_scope.
+Local Open Scope pg_scope.
 
 Definition get_new_vertex : program state Z := {|
   nrm := fun s1 n s2 =>
     s2.(max_v) = s1.(max_v) + 1 /\
     s2.(max_e) = s1.(max_e) /\
-    n = max_v s2;
+    n = s2.(max_v);
   err := fun s1 => False (* no error case *)
 |}.
 
-Definition pregraph_add_vertex {T} (g: @pg_nfa T) (v: Z) : program state (@pg_nfa T) := {|
-  nrm :=
-    fun s1 g' s2 =>
-    let g1 := g.(pg) in
-    let g2 := g'.(pg) in
-    s1 = s2 /\
-    g2.(evalid) = g1.(evalid) /\
-    g2.(vvalid) = addValidFunc v g1.(vvalid) /\
-    g2.(src) = g1.(src) /\
-    g2.(dst) = g1.(dst);
-  err := fun s1 => v > s1.(max_v) + 1
-  (* error if new vertex label mismatches current state *)
+Definition G_add_vertex {T} (g: pg_nfa T) (n: Z):
+  program state (pg_nfa T) :=
+{|
+  nrm := fun s1 g0 s2 => add_vertex g n g0 /\ s1 = s2;
+  err := fun _ => n ∈ g.(pg).(vvalid);
 |}.
-
-Definition pregraph_add_new_vertex {T} (g: @pg_nfa T) : program state (@pg_nfa T) :=
-  n <- get_new_vertex ;;
-  pregraph_add_vertex g n.
 
 Definition get_new_edge : program state Z := {|
   nrm :=
@@ -49,175 +41,99 @@ Definition get_new_edge : program state Z := {|
   err := fun s1 => False (* no error case *)
 |}.
 
-(* add_vertex relation (g1 v g2)*)
-
-Definition pregraph_add_edge {T} (g: @pg_nfa T) (e: Z) (s t: Z) : program state (@pg_nfa T) := {|
+Definition G_add_edge {T} (g: pg_nfa T) (e x y: Z) t: program state (pg_nfa T) := {|
   nrm :=
-    fun s1 g' s2 =>
-    let g1 := g.(pg) in
-    let g2 := g'.(pg) in
-    s1 = s2 /\
-    g2.(vvalid) = g1.(vvalid) /\
-    g2.(evalid) = addValidFunc e g1.(evalid) /\
-    g2.(src) = updateEdgeFunc g1.(src) e s /\
-    g2.(dst) = updateEdgeFunc g1.(dst) e t;
+    fun s1 g0 s2 =>
+      add_edge g e x y t g0 /\ s1 = s2;
   err :=
-    fun s1 =>
-    let g1 := g.(pg) in
-    exists e',
-    g1.(vvalid) s /\ g1.(vvalid) t /\
-    g1.(evalid) e' /\
-    g1.(src) e' = s /\
-    g1.(dst) e' = t
-  (* error if edge exists *)
+    fun _ => e ∈ g.(pg).(evalid);
 |}.
 
-Definition pregraph_add_new_edge {T} (g: @pg_nfa T) (s t: Z) : program state (@pg_nfa T) :=
-  n <- get_new_edge ;;
-  pregraph_add_edge g n s t.
-
-Definition updateEdgeSymbol {T} (g: @pg_nfa T) (e: Z) (c: option T) : program state (@pg_nfa T) := {|
+Definition G_add_graph {T} (g1 g2: pg_nfa T): program state (pg_nfa T) := {|
   nrm :=
-    fun s1 g' s2 =>
-    s1 = s2 /\
-    g'.(symbol) = fun n => if Z.eqb e n then c else g.(symbol) n;
-  err := fun s1 => False
-|}.
-(* Relation *)
-
-Definition graph_union {T} (A B: @pg_nfa T) : program state pg_nfa := {|
-  nrm :=
-    fun s1 G s2 =>
-    s1 = s2 /\
-    G_union_rel A B G;
+    fun s1 g3 s2 =>
+      union_rel g1 g2 g3 /\ s1 = s2;
   err :=
-    fun s1 => vertex_overlap A B \/ edge_overlap A B \/ symbol_overlap A B
+    fun s1 => Sets_overlap g1.(pg).(vvalid) g2.(pg).(vvalid) \/
+              Sets_overlap g1.(pg).(evalid) g2.(pg).(evalid);
 |}.
-
-Definition nfa_to_elem {T} (sv ev: Z) (g: @pg_nfa T) : program state elem := {|
-  nrm :=
-    fun s1 E s2 =>
-    s1 = s2 /\
-    E = {|
-      startVertex := sv;
-      endVertex := ev;
-      graph := g
-    |};
-  err :=
-    fun s1 =>
-    ~ vvalid g.(pg) sv \/ ~ vvalid g.(pg) ev
-|}.
-
-(** *)
-
-Definition pregraph_add_whole_edge {T} (g: @pg_nfa T) (s t: Z)
-  (c: option T) : program state pg_nfa :=
-  e <- get_new_edge ;;
-  g1 <- pregraph_add_edge g e s t ;;
-  updateEdgeSymbol g1 e c.
 
 Inductive graph_construction_component {T} :=
-  | G (g: @pg_nfa T)
+  | G (g: pg_nfa T)
   | V (v: Z)
-  | E (v1 v2: Z) (sbl: option T).
+  | E (v1 v2: Z) (sbl: option (T -> Prop)).
 
-Definition pregraph_add_component {T} (g: @pg_nfa T)
-  (comp: graph_construction_component)
-  : program state pg_nfa :=
-  match comp with
-  | G g' => graph_union g g'
-  | V v => pregraph_add_vertex g v
-  | E v1 v2 sbl => pregraph_add_whole_edge g v1 v2 sbl
-  end
-.
+Fixpoint graph_constr_rec {T} (g0: pg_nfa T) (l: list graph_construction_component)
+: program state (pg_nfa T) :=
+  match l with
+  | nil => ret g0
+  | G g :: l0 => g1 <- G_add_graph g0 g;; graph_constr_rec g1 l0
+  | V v :: l0 => g1 <- G_add_vertex g0 v;; graph_constr_rec g1 l0
+  | E x y t :: l0 => e <- get_new_edge;;
+                     g1 <- G_add_edge g0 e x y t;;
+                     graph_constr_rec g1 l0
+  end.
 
-Fixpoint pregraph_merge_comp_list {T} (g: @pg_nfa T)
-  (l_comp: list graph_construction_component)
-  : program state pg_nfa :=
-  match l_comp with
-  | nil => return g
-  | cons comp l_comp' =>
-    g1 <- pregraph_add_component g comp ;;
-    pregraph_merge_comp_list g1 l_comp'
-  end
-.
+Definition graph_constr {T} (l: list graph_construction_component):
+  program state (pg_nfa T) :=
+  graph_constr_rec empty_nfa l.
+
+Definition ret_nfa {T: Type} (x y: Z) (g: pg_nfa T):
+  program state (elem T) :=
+  ret (Build_elem _ x y g).
 
 (** Regex operator definition (concat/union/star/...) *)
 
-Definition act_empty {T} : program state (@elem T) :=
+Definition act_empty {T}: program state (elem T) :=
   v1 <- get_new_vertex ;;
   v2 <- get_new_vertex ;;
-  g1 <- pregraph_merge_comp_list empty_nfa [V v1; V v2] ;;
-  nfa_to_elem v1 v2 g1.
+  g1 <- graph_constr [V v1; V v2] ;;
+  ret_nfa v1 v2 g1.
 
 (* match single char c *)
-Definition act_singleton {T} (c: option T) : program state elem :=
+Definition act_singleton {T} (t: option (T -> Prop)):
+  program state (elem T) :=
   v1 <- get_new_vertex ;;
   v2 <- get_new_vertex ;;
-  g1 <- pregraph_merge_comp_list empty_nfa [V v1; V v2; E v1 v2 c] ;;
-  nfa_to_elem v1 v2 g1.
+  g1 <- graph_constr [V v1; V v2; E v1 v2 t] ;;
+  ret_nfa v1 v2 g1.
 
 (* match A|B *)
-Definition act_union {T} (A B: @elem T) : program state elem :=
+Definition act_union {T} (A B: elem T) : program state (elem T) :=
   v1 <- get_new_vertex ;;
   v2 <- get_new_vertex ;;
-  g <- pregraph_merge_comp_list A.(graph) [G B.(graph);
-                                            V v1;
-                                            V v2;
-                                            E v1 A.(startVertex) epsilon;
-                                            E v1 B.(startVertex) epsilon;
-                                            E A.(endVertex) v2 epsilon;
-                                            E B.(endVertex) v2 epsilon] ;;
-  nfa_to_elem v1 v2 g.
-
-  (* 合并操作 get_new_edge, pregraph_add_edge, updateEdgeSymbol *)
-  (* graph_construction : list graph_construction_component -> program state graph *)
-  (* Inductive graph_construction_component :=  G (g: pg_nfa)
-                                              | V (v: Z)
-                                              | E (v1 v2: Z) (label: option ascii). *)
-  (* list gr_constr_comp -> Monad *)
+  g <- graph_constr  [G A.(graph);
+                      G B.(graph);
+                      V v1;
+                      V v2;
+                      E v1 A.(startVertex) epsilon;
+                      E v1 B.(startVertex) epsilon;
+                      E A.(endVertex) v2 epsilon;
+                      E B.(endVertex) v2 epsilon] ;;
+  ret_nfa v1 v2 g.
 
 (* match AB *)
-Definition act_concat {T} (A B: @elem T) : program state elem :=
-  g <- pregraph_merge_comp_list A.(graph) [G B.(graph);
-                                           E A.(endVertex) B.(startVertex) epsilon] ;;
-  nfa_to_elem A.(startVertex) B.(endVertex) g.
+Definition act_concat {T} (A B: elem T) : program state (elem T) :=
+  g <- graph_constr [G A.(graph);
+                     G B.(graph);
+                     E A.(endVertex) B.(startVertex) epsilon] ;;
+  ret_nfa A.(startVertex) B.(endVertex) g.
   
 (* match A* *)
-Definition act_star {T} (A: @elem T) : program state elem :=
-  let g := A.(graph) in
+Definition act_star {T} (A: elem T) : program state (elem T) :=
   v1 <- get_new_vertex ;;
   v2 <- get_new_vertex ;;
-  g1 <- pregraph_merge_comp_list g [V v1;
-                                    V v2;
-                                    E v1 A.(endVertex) epsilon;
-                                    E A.(endVertex) v2 epsilon;
-                                    E A.(endVertex) A.(startVertex) epsilon] ;;
-  nfa_to_elem v1 v2 g1.
-
-(* match A+ *)
-Definition act_plus {T} (A: @elem T) : program state elem :=
-  let g := A.(graph) in
-  v1 <- get_new_vertex ;;
-  v2 <- get_new_vertex ;;
-  g1 <- pregraph_add_vertex g v1 ;;
-  g2 <- pregraph_add_vertex g1 v2 ;;
-  g3 <- pregraph_add_whole_edge g2 v1 A.(startVertex) epsilon ;;
-  g4 <- pregraph_add_whole_edge g3 A.(endVertex) v2 epsilon ;;
-  g5 <- pregraph_add_whole_edge g4 A.(endVertex) A.(startVertex) epsilon ;;
-  nfa_to_elem v1 v2 g5.
-
-(* match A? *)
-Definition act_question {T} (A: @elem T) : program state elem :=
-  let g := A.(graph) in
-  g1 <- pregraph_add_whole_edge g A.(startVertex) A.(endVertex) epsilon ;;
-  nfa_to_elem A.(startVertex) A.(endVertex) g1.
+  g1 <- graph_constr [G A.(graph);
+                      V v1; V v2;
+                      E v1 A.(endVertex) epsilon;
+                      E A.(endVertex) v2 epsilon;
+                      E A.(endVertex) A.(startVertex) epsilon] ;;
+  ret_nfa v1 v2 g1.
 
 (* Regex AST <-> NFA Monad *)
 
-Fixpoint regexToNFA {T} (r : reg_exp T) : program state elem :=
+Fixpoint regexToNFA {T} (r : reg_exp T) : program state (elem T) :=
   match r with
-  (** 2 vertices *)
   | EmptySet_r => act_empty
 
   | EmptyStr_r => act_singleton None
@@ -238,10 +154,3 @@ Fixpoint regexToNFA {T} (r : reg_exp T) : program state elem :=
     E <- regexToNFA r ;;
     act_star E
   end.
-
-End NoGraph_NFA_DEF.
-
-
-(** 1. st_nograph <-> regex *)
-
-(** NFA accepts a string ? *)
